program_logic/global_cmra.v
@@ -1,4 +1,4 @@
-Require Export program_logic.ownership program_logic.pviewshifts.
+Require Export algebra.iprod program_logic.ownership program_logic.pviewshifts.
 Import uPred.
 
 Definition gid := positive.
@@ -15,26 +15,41 @@ Definition to_globalC {Λ} {Δ : gid → iFunctor}
   iprod_singleton i {[ γ ↦ to_funC _ a ]}.
 Definition own {Λ} {Δ : gid → iFunctor}
     (i : gid) `{!InG Λ Δ i A} (γ : gid) (a : A) : iProp Λ (globalC Δ) :=
-  ownG (Σ:=globalC Δ) (iprod_singleton i {[ γ ↦ to_funC _ a ]}).
+  ownG (Σ:=globalC Δ) (to_globalC i γ a).
 
 Section global.
 Context {Λ : language} {Δ : gid → iFunctor} (i : gid) `{!InG Λ Δ i A}.
 Implicit Types a : A.
 
+(* Proeprties of to_globalC *)
+Lemma globalC_op γ a1 a2 :
+  to_globalC i γ (a1 ⋅ a2) ≡ to_globalC i γ a1 ⋅ to_globalC i γ a2.
+Proof.
+  rewrite /to_globalC iprod_op_singleton map_op_singleton.
+  apply iprod_singleton_proper, (fin_maps.singleton_proper (M:=gmap _)).
+  by rewrite /to_funC; destruct inG.
+Qed.
+
+Lemma globalC_validN n γ a :
+  ✓{n} (to_globalC i γ a) <-> ✓{n} a.
+Proof.
+  rewrite /to_globalC.
+  rewrite -iprod_validN_singleton -map_validN_singleton.
+  by rewrite /to_funC; destruct inG.
+Qed.
+
+(* Properties of own *)
+
 Global Instance own_ne γ n : Proper (dist n ==> dist n) (own i γ).
 Proof.
   intros m m' Hm; apply ownG_ne, iprod_singleton_ne, singleton_ne.
-  by rewrite /to_funC; destruct inG.
+  by rewrite /to_globalC /to_funC; destruct inG.
 Qed.
 
 Global Instance own_proper γ : Proper ((≡) ==> (≡)) (own i γ) := ne_proper _.
 
 Lemma own_op γ a1 a2 : own i γ (a1 ⋅ a2) ≡ (own i γ a1 ★ own i γ a2)%I.
-Proof.
-  rewrite /own -ownG_op iprod_op_singleton map_op_singleton.
-  apply ownG_proper, iprod_singleton_proper, (fin_maps.singleton_proper (M:=gmap _)).
-  by rewrite /to_funC; destruct inG.
-Qed.
+Proof. rewrite /own -ownG_op. apply ownG_proper, globalC_op. Qed.
 
 (* TODO: This also holds if we just have ✓a at the current step-idx, as Iris
    assertion. However, the map_updateP_alloc does not suffice to show this. *)
@@ -50,7 +65,7 @@ Proof.
     + simpl. move=>? [γ [-> ?]]. exists γ. done.
   - apply exist_elim=>m. apply const_elim_l.
     move=>[p ->] {P}. by rewrite -(exist_intro p).
-Qed.      
+Qed.
 
 Lemma always_own_unit γ m : (□ own i γ (unit m))%I ≡ own i γ (unit m).
 Proof.
@@ -59,10 +74,9 @@ Admitted.
 
 Lemma own_valid γ m : (own i γ m) ⊑ (✓ m).
 Proof.
-  rewrite /own ownG_valid; apply uPred.valid_mono.
-intros n ?.
-SearchAbout validN singletonM.
-Admitted.
+  rewrite /own ownG_valid. apply uPred.valid_mono=>n.
+  by apply globalC_validN.
+Qed.
 
 Lemma own_valid_r' γ m : (own i γ m) ⊑ (own i γ m ★ ✓ m).
 Proof. apply (uPred.always_entails_r' _ _), own_valid. Qed.
@@ -70,7 +84,6 @@ Proof. apply (uPred.always_entails_r' _ _), own_valid. Qed.
 Global Instance ownG_timeless γ m : Timeless m → TimelessP (own i γ m).
 Proof.
   intros. apply ownG_timeless.
-SearchAbout singletonM Timeless.
 Admitted.
 
 End global.
